Rust.fst
@@ -1,0 +1,29 @@
+module Rust
+
+let vec (a : Type0) = list a
+
+val length : #a:Type0 -> vec a -> Tot nat
+let length #a v = List.Tot.Base.length v
+
+val fold : #a:Type0 -> #b:Type0 -> (a -> b -> Tot a) -> a -> v:vec b -> Tot a (decreases v)
+let fold #a #b f x v = List.Tot.Base.fold_left f x v
+
+val index : #a:Type0 -> v:vec a -> i:nat{i < length v} -> Tot a
+let index #a v i = List.Tot.Base.index #a v i
+
+val enumerate : #a:eqtype -> v:vec a ->
+  Tot (vec (a & i:int))
+let enumerate #a v = List.Tot.Base.mapi (fun i e -> (e,i)) v
+
+val foldl :
+  #b:Type ->
+  v:vec b{length v > 0} ->
+  a:(i:nat{i < length v} -> Type) ->
+  a 0 ->
+  f:( i:nat{i < length v - 1} -> b -> a i -> Tot (a (i+1))) ->
+  Tot (a (length v - 1)) (decreases v)
+let foldl #b v a x f =
+  Lib.LoopCombinators.repeat_left 0 ((length v - 1))
+    a
+    (fun i acc -> f i (List.Tot.Base.index v i) acc)
+    x
